commutative expression theorem

xc/theorems.v
@@ -8,29 +8,32 @@ Module Theorems (M: MAPPING).
   Include BS.
 
 
-  Definition comm_exp (e : exp) : Prop := 
+  Definition is_comm_exp (e : exp) : Prop := 
     match e with 
-    | exp_app_1 e1 e2 => forall id ss vtIn nval vtOut, 
+    | exp_app_2 e1 e2 e3 => forall id ss vtIn nval vtOut, 
       <[id | ss | vtIn | e]> ==> <[nval | vtOut]> 
       <->
-      <[id | ss | vtIn | (exp_app_1 e2 e1)]> ==> <[nval | vtOut]> 
+      <[id | ss | vtIn | (exp_app_2 e1 e3 e2)]> ==> <[nval | vtOut]> 
     | _ => False
     end.
 
-  Fixpoint swap (e: exp) : exp :=
+  Fixpoint swap (e commExp : exp) : exp :=
     match e with 
     | exp_var _ => e
-    | exp_app_1 e1 e2 => 
-      if comm_exp (e) 
-        then exp_app_1 (swap e2) (swap e1)
-        else exp_app_1 (swap e1) (swap e2)
-    | exp_app_2 e1 e2 e3 => exp_app_2 (swap e1) (swap e2) (swap e3) 
-    | exp_app_3 e1 e2 e3 e4 => exp_app_3 (swap e1) (swap e2) (swap e3) (swap e4) 
-    | exp_val s e1 e2 => exp_val s (swap e1) (swap e2) 
+    | exp_app_1 e1 e2 => exp_app_1 (swap e1 commExp) (swap e2 commExp)
+    | exp_app_2 e1 e2 e3 => exp_app_2 (swap e1 commExp) (swap e2 commExp) (swap e3 commExp) 
+    | exp_app_3 e1 e2 e3 e4 => exp_app_3 (swap e1 commExp) (swap e2 commExp) (swap e3 commExp) (swap e4 commExp) 
+    | exp_val s e1 e2 => exp_val s (swap e1 commExp) (swap e2 commExp) 
     | exp_literal _ => e
     | exp_nvalue _ => e
     end.
 
-  Theorem use_comm : forall id ss vtIn nval vtOut exp,
+  Theorem use_comm : forall commExp,
+    is_comm_exp commExp ->
+    forall id ss vtIn nval vtOut exp,
+      <[id | ss | vtIn | exp]> ==> <[nval | vtOut]>
+      <->
+      <[id | ss | vtIn | swap exp commExp]> ==> <[nval | vtOut]>.
+  Admitted.
 
 End Theorems.
